theories/heap_lang/proofmode.v
@@ -2,7 +2,7 @@ From iris.program_logic Require Export weakestpre total_weakestpre.
 From iris.program_logic Require Import atomic.
 From iris.proofmode Require Import coq_tactics reduction.
 From iris.proofmode Require Export tactics.
-From iris.heap_lang Require Export tactics lifting.
+From iris.heap_lang Require Export tactics lifting array.
 From iris.heap_lang Require Import notation.
 Set Default Proof Using "Type".
 Import uPred.
